examples/low-level/example1.fst
@@ -26,5 +26,6 @@ let increment r =
   write r (oldv + 1)
 
 (*ideally, the refExistsInMem clauses should not be needed in the postcondition*)
-val increment2 : r:(ref int) -> SST unit  (fun m -> (refExistsInMem r m)==true) (fun m0 a m1 -> (refExistsInMem r m0) /\ (refExistsInMem r m1) /\ (loopkupRef r m1 = (loopkupRef r m0) + 1))
+val increment2 : r:(ref int) -> SST unit  (fun m -> (refExistsInMem r m)==true)
+(fun m0 a m1 -> (refExistsInMem r m0) /\ (refExistsInMem r m1) /\ (loopkupRef r m1 = (loopkupRef r m0) + 1))
 let increment2 r = admit ()
